***
### Exercise 3.1-1
Let f(n) and g(n) be asymptotically nonnegative functions. Using the basic definition of Θ-notation, prove that max(f(n), g(n)) = Θ(f(n)+g(n)).
### `Answer`
By the definition of Θ-notation, we can write  
0 <= c1(f(n) + g(n)) <= max(f(n), g(n)) <= c2(f(n) + g(n))  
To prove this, all the inequalities need to hold true.  
As the max of two function cannot be greater than the sum of two, so c2 = 1.  
Max of two function cannot be less than average of two, so c1 = 1/2.  
And 0 <= c1(f(n) + g(n)) as the functions are nonnegative.  

***
### Exercise 3.1-2
Show that for any real constants a and b, where b > 0,
(n + a)<sup>b</sup> = Θ(n<sup>b</sup>).
### `Answer`
Here (n + a) <= 2n, when |a| <= n and (n + a) >= n/2, when |a| <= n/2.  
So n >= 2a  
So we can write,  
0 <= n/2 <= (n + a) <= 2n  
Now raising to the power b, we get  
0 <= (n/2)<sup>b</sup> <= (n + a)<sup>b</sup> <= (2n)<sup>b</sup>  
0 <= (1/2)<sup>b</sup>n<sup>b</sup> <= (n + a)<sup>b</sup> <= 2<sup>b</sup>n<sup>b</sup>  
Comparing this with 0 <= c1n<sup>b</sup> <= (n + a)<sup>b</sup> <= c2n<sup>b</sup>, we get  
c1 = (1/2)<sup>b</sup> , c2 = 2<sup>b</sup> and n<sub>0</sub> = 2a  
Therefore (n + a)<sup>b</sup> = Θ(n<sup>b</sup>).  

***
### Exercise 3.1-3
