***
### Exercise 3.2-1
Show that if f(n) and g(n) are monotonically increasing functions, then so are the functions f(n) + g(n) and f (g(n)), and if f(n) and g(n) 
are in addition nonnegative, then f(n) 路 g(n) is monotonically increasing.
### `Answer`
Given that f(n) and g(n) are monotonically increasing functions, So  
f(n) <= f(n+1) &nbsp; &nbsp; &nbsp; &nbsp; (1)  
g(n) <= g(n+1) &nbsp; &nbsp; &nbsp; &nbsp; (2)  
Adding eqn. (1) and (2), we get  
f(n) + g(n) <= f(n+1) + g(n+1)  
Therefore f(n) + g(n) is monotonically increasing function.  
Since, g(n) <= g(n+1) and f(n) is a monotonically increasing function.  
So, f(g(n)) <= f(g(n+1))  
Therefore f(g(n)) is a monotonically increasing function.  
  
Given f(n) >=0 and g(n) >= 0  
Then multiplying eqn. (1) and (2) results into  
f(n) 路 g(n) <= f(n+1) 路 g(n+1)  
Therefore f(n) 路 g(n) is monotonically increasing.

***
