***
### Exercise 4.3-1
Show that the solution of T(n) = T(n−1) + n is O(n<sup>2</sup>).
### `Answer`
*T(n) = T(n-1) + n  
To show: T(n) <= cn<sup></sup>  
By substitution method, we can write  
T(n) <= c(n-1)<sup>2</sup> + n  
T(n) <= c(n<sup>2</sup> -2n + 1) + n  
T(n) <= cn<sup>2</sup> - 2cn + c + n  
T(n) <= cn<sup>2</sup> + (1 - 2c)n + c  
So T(n) = O(n<sup>2</sup>) when n>1 and c>1.  
**OR**  
T(n) = T(n-1) + n  
T(n) = T(n-2) + (n-1) + n  
T(n) = T(n-3) + (n-2) + (n-1) + n  
T(n) = T(0) + 1 + 2 + . . . + n  
T(n) = T(0) + n(n+1)/2  
T(n) = O(1) + O(n<sup>2</sup>)  
T(n) = O(n<sup>2</sup>)*  

***
### Exercise 4.3-2
Show that the solution of T(n) = T(⌈n/2⌉) + 1 is O(lgn).
### `Answer`
*T(n) = T(⌈n/2⌉) + 1  
To show: T(n) <= clgn  
By substitution method, we can write  
T(n) <= clg(⌈n/2⌉) + 1  
T(n) <= clg(n/2 + 1) + 1  
T(n) <= clg((n+2)/2) + 1  
T(n) <= clg(n+2) - c + 1  
Which is not satisfying the case  
So Lets assume T(n) <= clg(n-b)  
So, T(n) <= clg(⌈n/2⌉ - b) + 1  
T(n) <= clg(n/2 -b + 1) + 1  
T(n) <= clg((n - 2b + 2)/2) + 1  
&nbsp; &nbsp; &nbsp; = clg(n - 2b + 2) - c + 1  
&nbsp; &nbsp; &nbsp; = clg(n - b - (b - 2)) - c + 1  
&nbsp; &nbsp; &nbsp; <= clg(n-b) holds for b>=2, c>=1 and n>b.*  

***
### Exercise 4.3-3
We saw that the solution of T(n) = 2T(⌊n/2⌋) + n is O(nlgn). Show that the solution of this recurrence is also Ω(nlgn). Conclude that the solution is Θ(nlgn).
### `Answer`
*T(n) = 2T(⌊n/2⌋) + n  
To show: T(n) >= cnlgn  
By substitution method, we can write  
T(n) >= 2c(⌊n/2⌋)lg(⌊n/2⌋) + n  
&nbsp; &nbsp; &nbsp; &nbsp;>= 2c(n/2 - 1)lg(n/2 - 1) + n  
&nbsp; &nbsp; &nbsp; &nbsp; = c(n-2){lg(n-2) - lg2} + n  
&nbsp; &nbsp; &nbsp; &nbsp; = c(n-2)lg(n-2) - c(n-2) + n  
This is not satisfying the above substitution.  
Now lets assume T(n) >= c(n+b)lg(n+b) for all n>n<sub>0</sub> where b,c,n<sub>0</sub> > 0.  
T(n) >= 2c(⌊n/2⌋ + b)lg(⌊n/2⌋ + b) + n  
&nbsp; &nbsp; &nbsp; &nbsp; = 2c(n/2 + b - 1)lg(n/2 + b - 1) + n  
&nbsp; &nbsp; &nbsp; &nbsp; = c(n + 2b - 2){lg(n + 2b - 2) - 1} + n  
&nbsp; &nbsp; &nbsp; &nbsp; = c(n + d)lg(n + d) - c(n + d) + n ,where d = 2b - 2  
&nbsp; &nbsp; &nbsp; &nbsp; = c(n + d)lg(n + d) + n - cd - cn  
&nbsp; &nbsp; &nbsp; &nbsp;>= c(n + d)lg(n + d)  holds when n - cd - cn >= 0.  
So T(n) = Ω(nlgn)  
Now since T(n) = Ω(nlgn) and T(n) = O(nlgn)  
Therefore T(n) = Θ(nlgn).*  

***
