***
### Exercise 2.3-1
Using Figure 2.4 as a model, illustrate the operation of merge sort on the array A = [3, 41, 52, 26, 38, 57, 9, 49].
### `Answer`
![pic](./pics/2.png)

***
### Exercise 2.3-2
Rewrite the MERGE procedure so that it does not use sentinels, instead stopping once either array L or R has had all its elements copied 
back to A and then copying the remainder of the other array back into A.
### `Answer`
```C++
void Merge(int arr[],int beg,int mid,int end){
  int temp[n];
  int i=beg, j=mid+1, k=beg;
  while(i<=mid && j<=end){
    if(arr[i]<=arr[j])
      temp[k++] = arr[i++];
    else
      temp[k++] = arr[j++];
  }
  while(i<=mid)
    temp[k++] = arr[i++];
  while(j<=end)
    temp[k++] = arr[j++];
  for(i=beg;i<=end;i++)
    arr[i] = temp[i];
}
```

***
### Exercise 2.3-3
Use mathematical induction to show that when n is an exact power of 2, the solution of the recurrence  
```
T(n) = 2           if n = 2  
      2T(n/2)+n    if n = 2^k , for k>1  
```
is T(n) = nlg(n).
### `Answer`
Let there exists a k > 1 such that T(2<sup>k</sup>) = 2<sup>k</sup>lg(2<sup>k</sup>). We need to prove that the formula holds for n = 2<sup>k+1</sup>.  
T(2<sup>k+1</sup>) = 2T(2<sup>k+1</sup>/2) + 2<sup>k+1</sup>  
 &nbsp; &nbsp; &nbsp; &nbsp; &nbsp; &nbsp;= 2T(2<sup>k</sup>) + 2\*2<sup>k</sup>  
 &nbsp; &nbsp; &nbsp; &nbsp; &nbsp; &nbsp;= 2\*2<sup>k</sup>lg(2<sup>k</sup>) + 2\*2<sup>k</sup>  
 &nbsp; &nbsp; &nbsp; &nbsp; &nbsp; &nbsp;= 2\*2<sup>k</sup>(lg(2<sup>k</sup>) + lg2)
 &nbsp; &nbsp; &nbsp; &nbsp; &nbsp; &nbsp;= 2<sup>k+1</sup>lg(2<sup>k+1</sup>)  
This induction holds for the above formula.  
Hence T(n) = nlg(n).

***
### Exercise 2.3-4
Insertion sort can be expressed as a recursive procedure as follows. In order to sort A[1..n], we recursively sort A[1..n -1] and then insert A[n] into the sorted array A[1..n - 1]. Write a recurrence for the running time of this recursive version of insertion sort.
### `Answer`
